# Proof by contrapositive

Look back at the definition of the **contrapositive** from Chapter 15. Do you notice something? The contrapositive always has the same truth value as the original conjecture $P \Rightarrow Q$. If one of them is true, the other is too. If one of them is false, the other is too.

Sometimes it can be easier to prove the contrapositive is true than to prove the original conjecture $P \Rightarrow Q$ is true. As they have identical truth values, this gives us a useful way of proving conjectures: If $T \Rightarrow S$ is true, then $P \Rightarrow Q$ is true. We use this method in this chapter. <br /> <br />

<div class="alert alert-warning" role="alert">
<strong>Why?</strong> 

To see why a conjecture $P \Rightarrow Q$ and its contrapositive $T \Rightarrow S$ have identical truth values, consider this: **Every element on the left hand side of a conjecture map *must* travel to the right hand side.** Therefore every element from both $P$ and $S$ must find a home in either $Q$ or $T$. 

A conjecture $P \Rightarrow Q$ asserts that *all* elements in $P$ end up in $Q$. Therefore if there are any elements in $T$, how did they get there? They of course came from the left hand side, but the conjecture maintains that they definitely didnâ€™t come from $P$, as all elements in $P$ went to $Q$. Therefore, if the conjecture $P \Rightarrow Q$ is true, then any element in $T$ must have come from $S$.

Proof by contrapositive exploits this fact, proving the every element in $P$ goes to $Q$ by proving that every element in $T$ started out in $S$ (or simply $T \Rightarrow S$ proves $P \Rightarrow Q$).

</div>


## Steps

1. Write the conjecture $P \Rightarrow Q$ in the form **If...then...**.
2. Write the contrapositive $T \Rightarrow S$ in the form **If...then...**.
3. Prove $T \Rightarrow S$.
4. This proves $P \Rightarrow Q$.

## Formal definition

To prove conjecture "If $P$ then $Q$" by contrapositive, show that

<center>

$T \Rightarrow S$

</center>

where $T \Rightarrow S$ is the contrapositive of the original conjecture.

## Conjectures

<div class="alert alert-info" role="alert">
```{exercise}
Use the following examples to practise proof by contrapositive. Try proving them using a direct proof too.

(\#cnj:xats): If $a^2+b^2$ is odd and $a$ and $b$ both integers, then one of $a$ or $b$ is even.
  
(\#cnj:xat): Every multiple of $3$ can be written as the sum of three consecutive integers

(\#cnj:xes): If $a, b$ are both even, then the sum of $a$ and $b$ is even.

(\#cnj:xian): The product of two non-integers is never an integer. (This was Conjecture 11.10.)

``` 
</div> 

<!-- *** -->

<!-- ***Solutions:*** -->

<!-- *** -->

<!-- Conjecture \@ref(cnj:xat): The conjecture is already in the form "If...then...". To prove this using a direct proof would require us to set $a^2 + b^2$ equal to $2k+1, k \in \mathbb Z$ (as we're told that it's odd) and then doing some crazy algebra involving three variables.  -->

<!-- But a proof by contrapositive here is very quick, so we'll use that: -->

<!-- ```{proof}  -->
<!-- The contrapositive of the conjecture is "If both of $a$ or $b$ is odd, then $a^2+b^2$ is even". -->

<!-- W.l.o.g. let $a$ be odd, so $b$ is even. We have, -->
<!-- \begin{align} -->
<!--     a &= 2k +1 \\ -->
<!--     b &= 2l -->
<!-- \end{align} -->
<!-- where $k,l \in \mathbb Z$. -->

<!-- Thus -->
<!-- \begin{align} -->
<!--     a^2 + b^2 &= (2k +1)^2 + (2k)^2 \\ -->
<!--     &= 4k^2 +4k + 1 + 4k^2 \\ -->
<!--     &= 8k^2 +4k + 1 \\ -->
<!--     &= 2(4k^2 +2k) + 1 \\ -->
<!-- \end{align} -->
<!-- which is clearly odd. -->

<!-- We have proved the contrapositive, $T \Rightarrow S$. Thus $P\Rightarrow Q$ is proved. -->
<!-- ``` -->

<!-- *** -->

<!-- Conjecture \@ref(cnj:xes):  -->

<!-- *** -->

<!-- Conjecture \@ref(cnj:xats):  -->

<!-- *** -->

<!-- Conjecture \@ref(cnj:xian): Rewritten, this conjecture becomes "If $a,b \notin \mathbb Z$, then $ab \notin \mathbb Z$". This conjecture is false, but I know many students struggle to see that immediately. So instead, consider the contrapositive of this conjecture: "If $ab \in \mathbb Z$, then at least one of $a$ or $b$ are integers". But it's easy to find counterexample to this. For example, let $ab = 1 = \frac{3}{5} \times \frac{5}{3}$. Or let $ab = 2 = \sqrt{2} \times \sqrt{2}$. As we've found counterexamples to the contrapositive, we know the original conjecture is false too.  -->

<!-- The counterexamples we found against the contrapositive can be reworked to give us counterexamples against the original conjecture: $a = b = \sqrt{2} \notin \mathbb Z$ but $ab = \sqrt{2} \times \sqrt{2} = 2 \in \mathbb Z$. -->

<!-- *** -->

<div class="alert alert-info" role="alert">
```{exercise}
This exercise will be uploaded at the start of our next class.

```
</div> 

