
\begin{equation} 
  f\left(k\right) = \binom{n}{k} p^k\left(1-p\right)^{n-k}
  (\#eq:binom)
\end{equation}

\begin{equation} 
  f\left(k\right) = \binom{n}{k} p^k\left(1-p\right)^{n-k}
\end{equation}

\begin{align}
a_1& =b_1+c_1\\
a_2& =b_2+c_2-d_2+e_2\\
\mathbb R
\end{align}

\begin{equation}
y = mx+b
\end{equation}

\begin{exercise} 
  \item One
\end{exercise}

```{theorem}
Here is my theorem.
```

```{lemma}
Here is my lemma
```

```{corollary}
Here is my corollary
```

```{proposition}
Here is my proposition
```

```{conjecture}
Here is my conjecture
```

```{definition}
Here is my definition
```

```{example}
Here is my example
```

```{exercise}
Here is my exercise.
```
